```
import java.util.Scanner;

public class Main {

	public static void main(String[] args) {
		
		Scanner sc = new Scanner(System.in);
		int D = sc.nextInt();
		int K = sc.nextInt();
		
		int a, b, i;
		int[] F = new int[D];
		F[1] = 1;
		F[2] = 1;
		
		for(i = 3; i < D; i++) {
			F[i] = F[i-2] + F[i-1];
		}
		
		for(a = 1; a < K; a++) {
			if((K - F[D-2] * a) % F[D-1] == 0) {
				b = (K - F[D-2] * a) / F[D-1];
				System.out.println(a);
				System.out.println(b);
			}
		}
		
	}	
}
```

<br>

결과 : 정답
